Restructure sections, add homomorphisms

groups.v
@@ -34,12 +34,15 @@ Section group_definitions.
 
 End group_definitions.
 
-Section group_laws.
+
+Section groups.
 
   Variables (A : Set) (op : A -> A -> A) (inv : A -> A) (zero : A).
   Variable (Group : is_group A op inv zero).
 
   Notation "x <*> y" := (op x y) (at level 50, left associativity).
+
+  Section group_laws.
 
   Lemma inverse1 (a: A): a <*> (inv a) = zero.
     unfold is_group, is_inverse in Group.
@@ -80,12 +83,6 @@ Section group_laws.
   Lemma group_assoc: forall a b c, (a <*> b) <*> c = a <*> (b <*> c).
     destruct Group as [[Assoc _] _]; auto.
   Qed.
-
-  Hint Rewrite inverse1.
-  Hint Rewrite inverse2.
-  Hint Rewrite group_assoc.
-  Hint Rewrite group_zero_l.
-  Hint Rewrite group_zero_r.
 
   Lemma group_cancel_l: forall a b c, op a b = op a c -> b = c.
     intros a b c OpABEqOpAC.
@@ -145,59 +142,6 @@ Section group_laws.
     symmetry; assumption.
   Qed.
 
-  Hint Rewrite inverse_cancel.
-
-  (* subgroup_mem is a characteristic function.  not sure if it will need to
-     be A -> Prop instead of a -> bool. *)
-  Definition is_subgroup (H: A -> bool) :=
-    (* 0 is a subgroup member *)
-    H zero = true /\
-    (* subgroup is closed under operation *)
-    (forall a b, H a = true /\ H b = true -> H (a <*> b) = true) /\
-    (* if an element is in the subgroup, its inverse is too *)
-    (forall a, H a = true -> H (inv a) = true).
-
-  Definition is_mem (mem: A -> bool) (a : A) := mem a = true.
-
-  (* c \in aH if b \in H such that ab = c, b = a^{-1}c *)
-  Definition left_coset (a: A) (H: A -> bool) := fun c => H ((inv a) <*> c).
-  (* c \in Ha if b \in H such that ba = c, b = c a^{-1} *)
-  Definition right_coset (H: A -> bool) (a: A) := fun c => H (c <*> (inv a)).
-
-  Lemma subgroup_op_closed: forall a b H,
-      is_subgroup H -> is_mem H a -> is_mem H b -> is_mem H (op a b).
-  Proof.
-    intros a b H.
-    unfold is_subgroup.
-    intros [_ [H_closed _]].
-    intros Ha Hb.
-    apply H_closed.
-    auto.
-  Qed.
-
-  Lemma subgroup_inverse1: forall a H, is_subgroup H -> is_mem H a -> is_mem H (inv a).
-    intros a H IsSubgroup.
-    unfold is_subgroup in IsSubgroup.
-    destruct IsSubgroup as [_ [_ Inverse]].
-    apply Inverse.
-  Qed.
-
-  Lemma subgroup_inverse2: forall a H, is_subgroup H -> is_mem H (inv a) -> is_mem H a.
-    intros a H IsSubgroup H_inv_a.
-    rewrite <- inverse_cancel.
-    apply subgroup_inverse1.
-    auto.
-    assumption.
-  Qed.
-
-  Lemma subgroup_inverse: forall a H, is_subgroup H -> is_mem H (inv a) <-> is_mem H a.
-  Proof.
-    intros.
-    split.
-    apply subgroup_inverse2; auto.
-    apply subgroup_inverse1; auto.
-  Qed.
-
   Lemma inverse_apply: forall a b, inv (a <*> b) = inv b <*> inv a.
   Proof.
     intros a b.
@@ -209,166 +153,6 @@ Section group_laws.
     rewrite inverse1.
     rewrite group_zero_l.
     rewrite inverse1; reflexivity.
-  Qed.
-
-  Lemma coset_intersection_helper_1:
-    forall a b H,
-      is_subgroup H ->
-      (exists x, is_mem (right_coset H a) x /\  is_mem (right_coset H b) x) ->
-      exists h1 h2, is_mem H h1 /\ is_mem H h2 /\ a = op (op (inv h1) h2) b.
-    intros a b H IsSubgroup [x [Ha_x Hb_x]].
-    unfold is_mem, right_coset, left_coset in Ha_x, Hb_x.
-    exists (x <*> inv a), (x <*> inv b).
-    split; [assumption | split; [assumption | auto]].
-    rewrite inverse_apply.
-    repeat rewrite group_assoc.
-    rewrite <- (group_assoc (inv x) _ _).
-    repeat rewrite inverse2.
-    rewrite inverse_cancel.
-    repeat rewrite group_zero_r.
-    reflexivity.
-  Qed.
-
-  Lemma subgroup_op_non_member_right: forall a b H,
-      is_subgroup H -> H a = true /\ H b = false -> H (a <*> b) = false.
-    intros a b H IsSubgroup Ha_true.
-    (* Suppose ab were in the subgroup.  Then a^{-1} ab would be in the subgroup, so b is in the subgroup.
-         contradiction *)
-    destruct (bool_dec (H (a <*> b)) false) as [Hab_false | Hab_true].
-    assumption.
-    destruct Ha_true as [Ha_true Hb_false].
-    apply not_false_is_true in Hab_true.
-    apply (subgroup_op_closed (inv a) _ H IsSubgroup) in Hab_true.
-    rewrite <- group_assoc in Hab_true.
-    rewrite inverse2 in Hab_true.
-    rewrite group_zero_l in Hab_true.
-    unfold is_mem in Hab_true.
-    rewrite Hb_false in Hab_true.
-    contradict Hab_true.
-    auto.
-    apply (subgroup_inverse _ _ IsSubgroup).
-    auto.
-  Qed.
-
-  Lemma subgroup_op_non_member_left: forall a b H,
-      is_subgroup H -> H a = false /\ H b = true -> H (a <*> b) = false.
-    intros a b H IsSubgroup [Ha_false Hb_true].
-    (* not sure if there is a clever way to use right, so we just duplicate the logic above (for now) *)
-    (* Suppose ab were in the subgroup.  Then abb^{-1} would be in the subgroup, so a is in the subgroup.
-         contradiction *)
-    destruct (bool_dec (H (a <*> b)) false) as [Hab_false | Hab_true].
-    assumption.
-    apply not_false_is_true in Hab_true.
-    apply (subgroup_op_closed _ (inv b) H IsSubgroup) in Hab_true.
-    autorewrite with core in Hab_true.
-    unfold is_mem in Hab_true.
-    rewrite Ha_false in Hab_true.
-    contradict Hab_true.
-    auto.
-    apply (subgroup_inverse _ _ IsSubgroup).
-    auto.
-  Qed.
-
-  Lemma subgroup_mem_l:
-    forall a b H, is_subgroup H -> H a = true -> H (a <*> b) = H b.
-    intros a b H IsSubgroup.
-    intros Hb_true.
-    (* want to reason like .... H b = true
-       If H a = true, then obviously since a is in the subgroup.
-       If H a = false, then...
-     *)
-    destruct (bool_dec (H b) true) as [Ha_true | Ha_false].
-    rewrite Ha_true; apply (subgroup_op_closed _ _ H IsSubgroup Hb_true Ha_true).
-    apply not_true_is_false in Ha_false.
-    rewrite Ha_false.
-    apply (subgroup_op_non_member_right a b H IsSubgroup).
-    auto.
-  Qed.
-
-  Lemma subgroup_mem_r:
-    forall a b H, is_subgroup H -> H b = true -> H (a <*> b) = H a.
-    intros a b H IsSubgroup.
-    intros Hb_true.
-    (* want to reason like .... H b = true
-       If H a = true, then obviously since a is in the subgroup.
-       If H a = false, then...
-     *)
-    destruct (bool_dec (H a) true) as [Ha_true | Ha_false].
-    rewrite Ha_true; apply (subgroup_op_closed _ _ H IsSubgroup Ha_true Hb_true).
-    apply not_true_is_false in Ha_false.
-    rewrite Ha_false.
-    apply (subgroup_op_non_member_left a b H IsSubgroup).
-    auto.
-  Qed.
-
-  Lemma subgroup_inverse_non_member1: forall a H, is_subgroup H -> H a = false -> H (inv a) = false.
-    intros a H IsSubgroup.
-    intros Ha_false.
-    destruct (bool_dec (H (inv a)) true) as [Ha_inv_true | Ha_inv_false].
-    apply (subgroup_inverse _ _ IsSubgroup) in Ha_inv_true.
-    rewrite inverse_cancel in Ha_inv_true.
-    unfold is_mem in Ha_inv_true.
-    rewrite Ha_false in Ha_inv_true.
-    contradict Ha_inv_true.
-    auto.
-    apply not_true_is_false in Ha_inv_false; auto.
-  Qed.
-
-  Lemma subgroup_inverse_non_member2: forall a H, is_subgroup H -> H (inv a) = false -> H a = false.
-    intros a H IsSubgroup.
-    intros Ha_inv_false.
-    apply (subgroup_inverse_non_member1 (inv a) H IsSubgroup) in Ha_inv_false.
-    rewrite <- (inverse_cancel a).
-    assumption.
-  Qed.
-
-  (* a in Hb -> Ha = Hb *)
-  Lemma coset_intersection:
-    forall a b H,
-      is_subgroup H ->
-      (exists x, is_mem (right_coset H a) x /\  is_mem (right_coset H b) x) ->
-      (forall c, (right_coset H a) c = (right_coset H b) c).
-    intros a b H IsSubgroup Intersection.
-    apply (coset_intersection_helper_1 a b H IsSubgroup) in Intersection.
-    destruct Intersection as [h1 [h2 [h1_Subgroup [h2_Subgroup a_definition]]]].
-    intros c.
-    unfold right_coset.
-    rewrite a_definition.
-    repeat rewrite inverse_apply.
-    rewrite inverse_cancel.
-    rewrite <- group_assoc.
-    apply (subgroup_inverse1 h2 H IsSubgroup) in h2_Subgroup.
-    apply (subgroup_op_closed (inv h2) h1 H IsSubgroup h2_Subgroup) in h1_Subgroup.
-    apply (subgroup_mem_r _ (inv h2 <*> h1) H IsSubgroup).
-    assumption.
-  Qed.
-
-  Lemma coset_reflexive: forall a H, is_subgroup H -> right_coset H a a = true.
-  Proof.
-    intros a H IsSubgroup.
-    unfold right_coset.
-    rewrite inverse1.
-    apply IsSubgroup.
-  Qed.
-
-  Theorem coset_representative:
-    forall a b H,
-      is_subgroup H -> right_coset H b a = true ->
-      forall c, right_coset H a c = right_coset H b c.
-  Proof.
-    intros a b H IsSubgroup.
-    intros Hb_a.
-    (* going to show that a is in both Ha Hb *)
-    remember (coset_reflexive a H IsSubgroup) as Ha_a.
-    apply (coset_intersection a b H IsSubgroup); auto.
-    exists a; auto.
-  Qed.
-
-  Theorem coset_mult: forall a b H, is_subgroup H -> is_mem H b -> is_mem (right_coset H a) (op b a).
-    intros a b H IsSubgroup Hb_true.
-    unfold right_coset, is_mem.
-    autorewrite with core.
-    auto.
   Qed.
 
   Lemma inverse_swap: forall a b c, a = op (inv b) c <-> op b a = c.
@@ -389,8 +173,6 @@ Section group_laws.
     assumption.
   Qed.
 
-  Hint Rewrite inverse_swap.
-
   Lemma inverse_zero : inv zero = zero.
     apply (group_cancel_l zero).
     rewrite inverse1.
@@ -398,138 +180,401 @@ Section group_laws.
     reflexivity.
   Qed.
 
+  End group_laws.
+
+  Hint Rewrite inverse_swap.
   Hint Rewrite inverse_zero.
+  Hint Rewrite inverse1.
+  Hint Rewrite inverse2.
+  Hint Rewrite group_assoc.
+  Hint Rewrite group_zero_l.
+  Hint Rewrite group_zero_r.
+  Hint Rewrite inverse_cancel.
+  Hint Rewrite inverse_apply.
 
-  Theorem coset_zero:
-    forall a H, is_subgroup H -> is_mem H a -> forall c, right_coset H a c = right_coset H zero c.
-  Proof.
-    intros a H IsSubgroup Ha_true.
-    (* WTS: everything in Ha can be represented by something in H *)
-    unfold right_coset.
-    intros c.
-    apply (subgroup_inverse _ _ IsSubgroup) in Ha_true.
-    rewrite (subgroup_mem_r _ _ H IsSubgroup).
-    autorewrite with core.
-    reflexivity.
-    auto.
-  Qed.
+  Section subgroups.
 
-  Definition is_normal_subgroup (H: A -> bool) :=
-    is_subgroup H /\ forall (a h : A), is_mem H h -> is_mem H (a <*> h <*> inv a).
+    (* subgroup_mem is a characteristic function.  not sure if it will need to
+     be A -> Prop instead of a -> bool. *)
+    Definition is_subgroup (H: A -> bool) :=
+      (* 0 is a subgroup member *)
+      H zero = true /\
+      (* subgroup is closed under operation *)
+      (forall a b, H a = true /\ H b = true -> H (a <*> b) = true) /\
+      (* if an element is in the subgroup, its inverse is too *)
+      (forall a, H a = true -> H (inv a) = true).
 
-  Lemma normal_subgroup_intro: forall a h H,
-      is_normal_subgroup H -> is_mem H h ->
-      is_mem H (a <*> h <*> inv a).
-    intros a h H IsNormalSubgroup h_Subgroup.
-    destruct IsNormalSubgroup as [IsSubgroup Normality].
-    apply Normality.
-    assumption.
-  Qed.
+    Definition is_mem (mem: A -> bool) (a : A) := mem a = true.
 
-  Lemma normal_subgroup_conjuation: forall a h H,
-      is_normal_subgroup H -> is_mem H h ->
-      is_mem H (a <*> h <*> inv a) <-> is_mem H ((inv a) <*> h <*> a).
-  Proof.
-    intros a h H IsNormalSubgroup h_Subgroup.
-    (* inv (a b) = inv b inv a *)
-    destruct IsNormalSubgroup as [IsSubgroup h_Membership].
-    split.
-    intros a_h_inv_a_Subgroup.
-    rewrite <- (inverse_cancel a) at 2.
-    apply (h_Membership (inv a)).
-    assumption.
-    intros inv_a_h_a_Subgroup.
-    apply h_Membership.
-    assumption.
-  Qed.
+    Lemma subgroup_op_closed: forall a b H,
+        is_subgroup H -> is_mem H a -> is_mem H b -> is_mem H (op a b).
+    Proof.
+      intros a b H.
+      unfold is_subgroup.
+      intros [_ [H_closed _]].
+      intros Ha Hb.
+      apply H_closed.
+      auto.
+    Qed.
 
-  Theorem normal_subgroup_membership_commutes : forall a b H,
-      is_normal_subgroup H -> H (a <*> b) = H (b <*> a).
-    intros a b H IsNormalSubgroup.
-    assert (is_subgroup H) as IsSubgroup. destruct IsNormalSubgroup; auto.
-    destruct (bool_dec2 (H a) true (H b) true) as
-        [[[[Ha_true Hb_true] | [Ha_false Hb_true]] |
-           [Ha_true Hb_false]] | [Ha_false Hb_false]].
-    assert (H b = true) as Hb_true2. assumption.
-    apply (subgroup_op_closed a b H IsSubgroup Ha_true) in Hb_true.
-    apply (subgroup_op_closed b a H IsSubgroup Hb_true2) in Ha_true.
-    unfold is_mem in Ha_true, Hb_true.
-    rewrite Ha_true, Hb_true.
-    reflexivity.
-    apply not_true_is_false in Ha_false.
-    rewrite (subgroup_op_non_member_left a _ _ IsSubgroup),
-            (subgroup_op_non_member_right _ a _ IsSubgroup).
-    reflexivity.
-    auto.
-    auto.
-    apply not_true_is_false in Hb_false.
-    rewrite (subgroup_op_non_member_left b _ _ IsSubgroup),
-            (subgroup_op_non_member_right _ b _ IsSubgroup).
-    reflexivity.
-    auto.
-    auto.
-    (* this is silly but I need this later I think *)
-    assert (is_normal_subgroup H) as IsNormalSubgroup2. assumption.
-    destruct (bool_dec (H (a <*> b)) true) as [Hab_true | Hab_false].
-    rewrite Hab_true; symmetry.
-    (* ab \in H, WTS ba in H.  a^{-1}aba \in H *)
-    apply (normal_subgroup_intro (inv a)) in Hab_true.
-    autorewrite with core in Hab_true.
-    rewrite <- group_assoc, inverse2, group_zero_l in Hab_true.
-    assumption.
-    assumption.
-    apply not_true_is_false in Hab_false.
-    destruct (bool_dec (H (b <*> a)) true) as [Hba_true | Hba_false].
-    (* ba \in H, WTS ab in H (contradiction). b^{-1}bab \in H  *)
-    destruct IsNormalSubgroup as [_ Normality].
-    apply (Normality (inv b) _) in Hba_true.
-    autorewrite with core in Hba_true.
-    rewrite <- group_assoc, inverse2, group_zero_l in Hba_true.
-    contradict Hba_true.
-    unfold is_mem.
-    apply not_true_iff_false.
-    assumption.
-    apply not_true_is_false in Hba_false.
-    rewrite Hab_false, Hba_false; reflexivity.
-  Qed.
+    Lemma subgroup_inverse1: forall a H, is_subgroup H -> is_mem H a -> is_mem H (inv a).
+      intros a H IsSubgroup.
+      unfold is_subgroup in IsSubgroup.
+      destruct IsSubgroup as [_ [_ Inverse]].
+      apply Inverse.
+    Qed.
 
-  Theorem normal_subgroup_left_coset_iff_right_coset : forall a H,
-      is_normal_subgroup H ->
-      forall c, left_coset a H c = right_coset H a c.
-  Proof.
-    intros a H IsNormalSubgroup.
-    assert (is_subgroup H) as IsSubgroup.  destruct IsNormalSubgroup; auto.
-    intros c.
-    unfold left_coset.
-    unfold right_coset.
-    apply normal_subgroup_membership_commutes.
-    assumption.
-  Qed.
+    Lemma subgroup_inverse2: forall a H, is_subgroup H -> is_mem H (inv a) -> is_mem H a.
+      intros a H IsSubgroup H_inv_a.
+      rewrite <- inverse_cancel.
+      apply subgroup_inverse1.
+      auto.
+      assumption.
+    Qed.
 
-  Lemma normal_subgroup_coset_op : forall a b c d H,
-      is_normal_subgroup H ->
-      is_mem (right_coset H a) c -> is_mem (right_coset H b) d -> is_mem (right_coset H (a <*> b)) (c <*> d).
-    intros a b c d H IsNormalSubgroup.
-    assert (is_subgroup H) as IsSubgroup.  destruct IsNormalSubgroup; auto.
-    unfold is_mem, right_coset.
-    intros c_Coset d_Coset.
-    rewrite (normal_subgroup_membership_commutes _ _ H IsNormalSubgroup) in c_Coset.
-    fold (is_mem H (inv a <*> c)) in c_Coset.
-    fold (is_mem H (d <*> inv b)) in d_Coset.
-    apply (subgroup_op_closed _ _ H IsSubgroup c_Coset) in d_Coset.
-    rewrite group_assoc in d_Coset.
-    rewrite <- (group_assoc c d _) in d_Coset.
-    unfold is_mem in d_Coset.
-    rewrite (normal_subgroup_membership_commutes (inv a) _ H IsNormalSubgroup) in d_Coset.
-    rewrite inverse_apply.
-    rewrite <- group_assoc.
-    assumption.
-  Qed.
+    Lemma subgroup_inverse: forall a H, is_subgroup H -> is_mem H (inv a) <-> is_mem H a.
+    Proof.
+      intros.
+      split.
+      apply subgroup_inverse2; auto.
+      apply subgroup_inverse1; auto.
+    Qed.
+
+    Lemma subgroup_op_non_member_right: forall a b H,
+        is_subgroup H -> H a = true /\ H b = false -> H (a <*> b) = false.
+      intros a b H IsSubgroup Ha_true.
+      (* Suppose ab were in the subgroup.  Then a^{-1} ab would be in the subgroup, so b is in the subgroup.
+         contradiction *)
+      destruct (bool_dec (H (a <*> b)) false) as [Hab_false | Hab_true].
+      assumption.
+      destruct Ha_true as [Ha_true Hb_false].
+      apply not_false_is_true in Hab_true.
+      apply (subgroup_op_closed (inv a) _ H IsSubgroup) in Hab_true.
+      rewrite <- group_assoc in Hab_true.
+      rewrite inverse2 in Hab_true.
+      rewrite group_zero_l in Hab_true.
+      unfold is_mem in Hab_true.
+      rewrite Hb_false in Hab_true.
+      contradict Hab_true.
+      auto.
+      apply (subgroup_inverse _ _ IsSubgroup).
+      auto.
+    Qed.
+
+    Lemma subgroup_op_non_member_left: forall a b H,
+        is_subgroup H -> H a = false /\ H b = true -> H (a <*> b) = false.
+      intros a b H IsSubgroup [Ha_false Hb_true].
+      (* not sure if there is a clever way to use right, so we just duplicate the logic above (for now) *)
+      (* Suppose ab were in the subgroup.  Then abb^{-1} would be in the subgroup, so a is in the subgroup.
+         contradiction *)
+      destruct (bool_dec (H (a <*> b)) false) as [Hab_false | Hab_true].
+      assumption.
+      apply not_false_is_true in Hab_true.
+      apply (subgroup_op_closed _ (inv b) H IsSubgroup) in Hab_true.
+      autorewrite with core in Hab_true.
+      unfold is_mem in Hab_true.
+      rewrite Ha_false in Hab_true.
+      contradict Hab_true.
+      auto.
+      apply (subgroup_inverse _ _ IsSubgroup).
+      auto.
+    Qed.
+
+    Lemma subgroup_mem_l:
+      forall a b H, is_subgroup H -> H a = true -> H (a <*> b) = H b.
+      intros a b H IsSubgroup.
+      intros Hb_true.
+      (* want to reason like .... H b = true
+       If H a = true, then obviously since a is in the subgroup.
+       If H a = false, then...
+       *)
+      destruct (bool_dec (H b) true) as [Ha_true | Ha_false].
+      rewrite Ha_true; apply (subgroup_op_closed _ _ H IsSubgroup Hb_true Ha_true).
+      apply not_true_is_false in Ha_false.
+      rewrite Ha_false.
+      apply (subgroup_op_non_member_right a b H IsSubgroup).
+      auto.
+    Qed.
+
+    Lemma subgroup_mem_r:
+      forall a b H, is_subgroup H -> H b = true -> H (a <*> b) = H a.
+      intros a b H IsSubgroup.
+      intros Hb_true.
+      (* want to reason like .... H b = true
+       If H a = true, then obviously since a is in the subgroup.
+       If H a = false, then...
+       *)
+      destruct (bool_dec (H a) true) as [Ha_true | Ha_false].
+      rewrite Ha_true; apply (subgroup_op_closed _ _ H IsSubgroup Ha_true Hb_true).
+      apply not_true_is_false in Ha_false.
+      rewrite Ha_false.
+      apply (subgroup_op_non_member_left a b H IsSubgroup).
+      auto.
+    Qed.
+
+    Lemma subgroup_inverse_non_member1: forall a H, is_subgroup H -> H a = false -> H (inv a) = false.
+      intros a H IsSubgroup.
+      intros Ha_false.
+      destruct (bool_dec (H (inv a)) true) as [Ha_inv_true | Ha_inv_false].
+      apply (subgroup_inverse _ _ IsSubgroup) in Ha_inv_true.
+      rewrite inverse_cancel in Ha_inv_true.
+      unfold is_mem in Ha_inv_true.
+      rewrite Ha_false in Ha_inv_true.
+      contradict Ha_inv_true.
+      auto.
+      apply not_true_is_false in Ha_inv_false; auto.
+    Qed.
+
+    Lemma subgroup_inverse_non_member2: forall a H, is_subgroup H -> H (inv a) = false -> H a = false.
+      intros a H IsSubgroup.
+      intros Ha_inv_false.
+      apply (subgroup_inverse_non_member1 (inv a) H IsSubgroup) in Ha_inv_false.
+      rewrite <- (inverse_cancel a).
+      assumption.
+    Qed.
+
+  End subgroups.
+
+  Section cosets.
+
+    (* c \in aH if b \in H such that ab = c, b = a^{-1}c *)
+    Definition left_coset (a: A) (H: A -> bool) := fun c => H ((inv a) <*> c).
+    (* c \in Ha if b \in H such that ba = c, b = c a^{-1} *)
+    Definition right_coset (H: A -> bool) (a: A) := fun c => H (c <*> (inv a)).
+
+    Lemma coset_intersection_helper_1:
+      forall a b H,
+        is_subgroup H ->
+        (exists x, is_mem (right_coset H a) x /\  is_mem (right_coset H b) x) ->
+        exists h1 h2, is_mem H h1 /\ is_mem H h2 /\ a = op (op (inv h1) h2) b.
+      intros a b H IsSubgroup [x [Ha_x Hb_x]].
+      unfold is_mem, right_coset, left_coset in Ha_x, Hb_x.
+      exists (x <*> inv a), (x <*> inv b).
+      split; [assumption | split; [assumption | auto]].
+      rewrite inverse_apply.
+      repeat rewrite group_assoc.
+      rewrite <- (group_assoc (inv x) _ _).
+      repeat rewrite inverse2.
+      rewrite inverse_cancel.
+      repeat rewrite group_zero_r.
+      reflexivity.
+    Qed.
+
+    (* a in Hb -> Ha = Hb *)
+    Lemma coset_intersection:
+      forall a b H,
+        is_subgroup H ->
+        (exists x, is_mem (right_coset H a) x /\  is_mem (right_coset H b) x) ->
+        (forall c, (right_coset H a) c = (right_coset H b) c).
+      intros a b H IsSubgroup Intersection.
+      apply (coset_intersection_helper_1 a b H IsSubgroup) in Intersection.
+      destruct Intersection as [h1 [h2 [h1_Subgroup [h2_Subgroup a_definition]]]].
+      intros c.
+      unfold right_coset.
+      rewrite a_definition.
+      repeat rewrite inverse_apply.
+      rewrite inverse_cancel.
+      rewrite <- group_assoc.
+      apply (subgroup_inverse1 h2 H IsSubgroup) in h2_Subgroup.
+      apply (subgroup_op_closed (inv h2) h1 H IsSubgroup h2_Subgroup) in h1_Subgroup.
+      apply (subgroup_mem_r _ (inv h2 <*> h1) H IsSubgroup).
+      assumption.
+    Qed.
+
+    Lemma coset_reflexive: forall a H, is_subgroup H -> right_coset H a a = true.
+    Proof.
+      intros a H IsSubgroup.
+      unfold right_coset.
+      rewrite inverse1.
+      apply IsSubgroup.
+    Qed.
+
+    Theorem coset_representative:
+      forall a b H,
+        is_subgroup H -> right_coset H b a = true ->
+        forall c, right_coset H a c = right_coset H b c.
+    Proof.
+      intros a b H IsSubgroup.
+      intros Hb_a.
+      (* going to show that a is in both Ha Hb *)
+      remember (coset_reflexive a H IsSubgroup) as Ha_a.
+      apply (coset_intersection a b H IsSubgroup); auto.
+      exists a; auto.
+    Qed.
+
+    Theorem coset_mult: forall a b H, is_subgroup H -> is_mem H b -> is_mem (right_coset H a) (op b a).
+      intros a b H IsSubgroup Hb_true.
+      unfold right_coset, is_mem.
+      autorewrite with core.
+      auto.
+    Qed.
+
+    Theorem coset_zero:
+      forall a H, is_subgroup H -> is_mem H a -> forall c, right_coset H a c = right_coset H zero c.
+    Proof.
+      intros a H IsSubgroup Ha_true.
+      (* WTS: everything in Ha can be represented by something in H *)
+      unfold right_coset.
+      intros c.
+      apply (subgroup_inverse _ _ IsSubgroup) in Ha_true.
+      rewrite (subgroup_mem_r _ _ H IsSubgroup).
+      autorewrite with core.
+      reflexivity.
+      auto.
+    Qed.
+
+  End cosets.
+
+  Section normal_subgroups.
+
+    Definition is_normal_subgroup (H: A -> bool) :=
+      is_subgroup H /\ forall (a h : A), is_mem H h -> is_mem H (a <*> h <*> inv a).
+
+    Lemma normal_subgroup_intro: forall a h H,
+        is_normal_subgroup H -> is_mem H h ->
+        is_mem H (a <*> h <*> inv a).
+      intros a h H IsNormalSubgroup h_Subgroup.
+      destruct IsNormalSubgroup as [IsSubgroup Normality].
+      apply Normality.
+      assumption.
+    Qed.
+
+    Lemma normal_subgroup_conjuation: forall a h H,
+        is_normal_subgroup H -> is_mem H h ->
+        is_mem H (a <*> h <*> inv a) <-> is_mem H ((inv a) <*> h <*> a).
+    Proof.
+      intros a h H IsNormalSubgroup h_Subgroup.
+      (* inv (a b) = inv b inv a *)
+      destruct IsNormalSubgroup as [IsSubgroup h_Membership].
+      split.
+      intros a_h_inv_a_Subgroup.
+      rewrite <- (inverse_cancel a) at 2.
+      apply (h_Membership (inv a)).
+      assumption.
+      intros inv_a_h_a_Subgroup.
+      apply h_Membership.
+      assumption.
+    Qed.
+
+    Theorem normal_subgroup_membership_commutes : forall a b H,
+        is_normal_subgroup H -> H (a <*> b) = H (b <*> a).
+      intros a b H IsNormalSubgroup.
+      assert (is_subgroup H) as IsSubgroup. destruct IsNormalSubgroup; auto.
+      destruct (bool_dec2 (H a) true (H b) true) as
+          [[[[Ha_true Hb_true] | [Ha_false Hb_true]] |
+            [Ha_true Hb_false]] | [Ha_false Hb_false]].
+      assert (H b = true) as Hb_true2. assumption.
+      apply (subgroup_op_closed a b H IsSubgroup Ha_true) in Hb_true.
+      apply (subgroup_op_closed b a H IsSubgroup Hb_true2) in Ha_true.
+      unfold is_mem in Ha_true, Hb_true.
+      rewrite Ha_true, Hb_true.
+      reflexivity.
+      apply not_true_is_false in Ha_false.
+      rewrite (subgroup_op_non_member_left a _ _ IsSubgroup),
+      (subgroup_op_non_member_right _ a _ IsSubgroup).
+      reflexivity.
+      auto.
+      auto.
+      apply not_true_is_false in Hb_false.
+      rewrite (subgroup_op_non_member_left b _ _ IsSubgroup),
+      (subgroup_op_non_member_right _ b _ IsSubgroup).
+      reflexivity.
+      auto.
+      auto.
+      (* this is silly but I need this later I think *)
+      assert (is_normal_subgroup H) as IsNormalSubgroup2. assumption.
+      destruct (bool_dec (H (a <*> b)) true) as [Hab_true | Hab_false].
+      rewrite Hab_true; symmetry.
+      (* ab \in H, WTS ba in H.  a^{-1}aba \in H *)
+      apply (normal_subgroup_intro (inv a)) in Hab_true.
+      autorewrite with core in Hab_true.
+      rewrite <- group_assoc, inverse2, group_zero_l in Hab_true.
+      assumption.
+      assumption.
+      apply not_true_is_false in Hab_false.
+      destruct (bool_dec (H (b <*> a)) true) as [Hba_true | Hba_false].
+      (* ba \in H, WTS ab in H (contradiction). b^{-1}bab \in H  *)
+      destruct IsNormalSubgroup as [_ Normality].
+      apply (Normality (inv b) _) in Hba_true.
+      autorewrite with core in Hba_true.
+      rewrite <- group_assoc, inverse2, group_zero_l in Hba_true.
+      contradict Hba_true.
+      unfold is_mem.
+      apply not_true_iff_false.
+      assumption.
+      apply not_true_is_false in Hba_false.
+      rewrite Hab_false, Hba_false; reflexivity.
+    Qed.
+
+    Theorem normal_subgroup_left_coset_iff_right_coset : forall a H,
+        is_normal_subgroup H ->
+        forall c, left_coset a H c = right_coset H a c.
+    Proof.
+      intros a H IsNormalSubgroup.
+      assert (is_subgroup H) as IsSubgroup.  destruct IsNormalSubgroup; auto.
+      intros c.
+      unfold left_coset.
+      unfold right_coset.
+      apply normal_subgroup_membership_commutes.
+      assumption.
+    Qed.
+
+    Lemma normal_subgroup_coset_op : forall a b c d H,
+        is_normal_subgroup H ->
+        is_mem (right_coset H a) c -> is_mem (right_coset H b) d -> is_mem (right_coset H (a <*> b)) (c <*> d).
+      intros a b c d H IsNormalSubgroup.
+      assert (is_subgroup H) as IsSubgroup.  destruct IsNormalSubgroup; auto.
+      unfold is_mem, right_coset.
+      intros c_Coset d_Coset.
+      rewrite (normal_subgroup_membership_commutes _ _ H IsNormalSubgroup) in c_Coset.
+      fold (is_mem H (inv a <*> c)) in c_Coset.
+      fold (is_mem H (d <*> inv b)) in d_Coset.
+      apply (subgroup_op_closed _ _ H IsSubgroup c_Coset) in d_Coset.
+      rewrite group_assoc in d_Coset.
+      rewrite <- (group_assoc c d _) in d_Coset.
+      unfold is_mem in d_Coset.
+      rewrite (normal_subgroup_membership_commutes (inv a) _ H IsNormalSubgroup) in d_Coset.
+      rewrite inverse_apply.
+      rewrite <- group_assoc.
+      assumption.
+    Qed.
+  End normal_subgroups.
+
+  Section homomorphisms.
+    Definition is_homomorphism (A: Set) op inv zero (B: Set) op' inv' zero' (h: A -> B) :=
+      is_group A op inv zero /\
+      is_group B op' inv' zero' /\
+      h zero = zero' /\
+      forall a b,
+        h (op a b) = op' (h a) (h b).
+
+    Lemma id_homomorphism : is_homomorphism A op inv zero A op inv zero (fun a => a).
+      unfold is_homomorphism.
+      auto.
+    Qed.
+
+    Lemma abelian_group_inv_homomorphism :
+      is_abelian_group A op inv zero ->
+      is_homomorphism A op inv zero A op inv zero (fun a => (inv a)).
+    Proof.
+      unfold is_abelian_group, is_commutative.
+      intros [_ IsCommutative].
+      unfold is_homomorphism.
+      split; [assumption | split; [assumption | split; [apply inverse_zero|auto]]].
+      intros a b.
+      rewrite IsCommutative, inverse_apply; reflexivity.
+    Qed.
+
+  End homomorphisms.
 
   (* Universe of quotient groups is the coset universe, e.g. A -> bool *)
 
+  Definition Coset (H: A -> bool) (a : A) : Set :=
+    is_group A op inv zero /\ is_normal_subgroup H.
+
+
   Definition quotient_group_zero (H : A -> bool) := H.
-    (* zero is coset based on subgroup membership *)
+  (* zero is coset based on subgroup membership *)
 
   Definition quotient_group_op (a b: (A -> bool)) :=
     (* a is one coset,
@@ -541,13 +586,9 @@ Section group_laws.
     a.
 
 
+
   (* theorem should show is_group holds for a given quotient_group *)
 
-End quotient_groups.
+End groups.
 
-
-(* ring zero *)
-(* ring id *)
-(* ring mult *)
-(* ring add *)
-Definition is_ring (A: Set) := A -> A -> (A -> A -> A) -> (A -> A -> A).
+Check Coset.
